
# P1 逻辑表达式等价证明

- 证明方法
	- 代数
	- 真值表

## Ex. 1

> $A\oplus B\oplus C = A\odot B\odot C$

$$
\begin{aligned}
A\oplus B\oplus C &= (A\oplus B)\oplus C \\
          &= (A\oplus B)C' + (A\oplus B)'C \\
          &= (A\odot B)'C' + (A\odot B)C \\
          &= A\odot B\odot C
\end{aligned}
$$

---

- $A \oplus B = \overline{A}B + A\overline{B}$
- $A \odot B = AB + \overline{A}\,\overline{B} = \overline{A \oplus B}$
- $A \oplus (B \oplus C) = (A \oplus B) \oplus C$

## Ex. 2

> $AB+A'C+B'C = AB+C$

$$
\begin{aligned}
AB+A'C+B'C &= AB+(A'+B')C \\
           &= AB+(AB)'C \\
           &= (AB+(AB)')(AB+C) \\
           &= 1(AB)+C \\
           &= AB +C
\end{aligned}
$$


